<!-- 05-07-22 -->
# Regla de la Potencia

[a)](#a) $y = x^3$ 

[b)](#b) $y = 5x^7$ 

[c)](#c) $y = 3x^8 + 4x$  

[d)](#d) $y = \frac{1}{5}x^5$  

[e)](#e) $y = \sqrt[7]{x}$  

[f)](#f) $y = \frac{1}{x^3}$  

$$y = ax^b => y' = abx^{b-1}$$ 

---

### a  

$y' = 3x^2$

---

### b

$y' = 35x^6$

---

### c

$y' = 24x^7 + 4x^0 = 24x^7 + 4$

---

### d

$y' = \frac{5}{5}x^4 = x^4$

---

### e

$y = x^\frac{1}{7}$

$y' = \frac{1}{7}x^{\frac{1}{7} - 1}$ 

$\frac{1- 7}{7} = \frac{-6}{7}$

$y' = \frac{x^\frac{-6}{7}}{7}$  

---

### d

$y = x^{-3}$

$y' = -3x^{-4}$

---
