<!-- 05-07-22 -->
# Derivadas

### Definicion de la derivada

$\displaystyle \lim_{\Delta{x} \to 0} \frac{f(x + \Delta{x}) - f(x)}{\Delta{x}}$ This ecuation is the same as $f'(p)$
\
\
\
Example: $f(x) = x^2 + 1$ when $x = 2$

$\displaystyle f'(2) = \lim_{\Delta{x} \to 0} \frac{f(2 + \Delta{x}) - f(2)}{\Delta{x}}$

$f(2 + \Delta{x}) = (2 + \Delta{x})^2 + 1$  
$f(2) = (2)^2 + 1 = 5$  
\
$\displaystyle = \lim_{\Delta{x} \to 0} \frac{(2 + \Delta{x})^2 + 1 - 5}{\Delta{x}}$  
$\displaystyle = \lim_{\Delta{x} \to 0} \frac{\cancel{4} + 4\Delta{x} + \Delta{x}^2 - \cancel{4}}{\Delta{x}}$  
$\displaystyle = \lim_{\Delta{x} \to 0} \frac{\cancel{\Delta{x}}(4 + \Delta{x})}{\cancel{\Delta{x}}} = \lim_{\Delta{x} \to 0}4 + \lim_{\Delta{x} \to 0}\Delta{x} = 4 + 0$  
$= 4$

